pancake/proofs/pan_simpProofScript.sml
@@ -2,11 +2,12 @@
   Correctness proof for pan_simp
 *)
 
-open preamble panLangTheory pan_simpTheory panSemTheory
+open preamble
+     panSemTheory pan_simpTheory
 
 val _ = new_theory "pan_simpProof";
 
-val _ = set_grammar_ancestry ["panLang", "pan_simp", "panSem"];
+val _ = set_grammar_ancestry  ["panSem", "pan_simp"];
 
 val s = ``s:('a,'ffi) panSem$state``
 
@@ -29,7 +30,6 @@ Proof
   fs [evaluate_def]
 QED
 
-
 Theorem evaluate_while_body_same:
   (!(s:('a,'b)state). evaluate (body,s) = evaluate (body',s)) ==>
   !(s:('a,'b)state). evaluate (While e body,s) = evaluate (While e body',s)
@@ -47,6 +47,21 @@ Proof
   every_case_tac >>
   imp_res_tac evaluate_clock >>
   fs [dec_clock_def]
+QED
+
+
+Theorem evaluate_while_no_error_imp:
+  eval s e = SOME (ValWord w) /\
+  w <> 0w /\ s.clock <> 0 /\
+  FST (evaluate (While e c,s)) <> SOME Error ==>
+  FST (evaluate (c,dec_clock s)) <> SOME Error
+Proof
+  rw [] >>
+  pop_assum mp_tac >>
+  once_rewrite_tac [evaluate_def] >>
+  TOP_CASE_TAC >> fs [] >>
+  pairarg_tac >> fs [] >> rveq >>
+  every_case_tac >> fs []
 QED
 
 Theorem evaluate_seq_assoc:
@@ -68,26 +83,19 @@ Proof
 QED
 
 
-Theorem eval_set_var_lookup_eq:
-  eval (s with locals := lcs |+ (v,value)) (Var v) =
-  SOME value
-Proof
-  rw [eval_def, FLOOKUP_UPDATE]
-QED
-
-Theorem evaluate_retcall_ret_to_tail_eq:
+Theorem evaluate_seq_call_ret_eq:
   !p s.
    FST (evaluate (p,s)) <> SOME Error ==>
-   evaluate (retcall_ret_to_tail p,s) = evaluate (p,s)
+   evaluate (seq_call_ret p,s) = evaluate (p,s)
 Proof
-  rw [retcall_ret_to_tail_def] >>
+  rw [seq_call_ret_def] >>
   every_case_tac >> fs [] >> rveq >>
   fs [evaluate_def] >>
   pairarg_tac >> fs [] >>
   every_case_tac >> fs [] >> rveq >>
   TRY (metis_tac [] >> NO_TAC) >>
   fs [empty_locals_def, set_var_def] >>
-  fs [eval_set_var_lookup_eq]
+  fs [eval_def, FLOOKUP_UPDATE]
 QED
 
 
@@ -100,10 +108,19 @@ Proof
   every_case_tac >> fs[]
 QED
 
+
+Theorem eval_seq_assoc_not_error:
+  FST (evaluate (p,s)) ≠ SOME Error ==>
+      FST (evaluate ((seq_assoc Skip p),s)) ≠ SOME Error
+Proof
+  rw [evaluate_seq_assoc] >>
+  rw [evaluate_def]
+QED
+
 val goal =
   ``λ(prog, s).
     FST (evaluate (prog,s)) <> SOME Error ==>
-    evaluate (retcall_elim prog, s) = evaluate (prog,s)``
+    evaluate (ret_to_tail prog, s) = evaluate (prog,s)``
 
 local
   val ind_thm = panSemTheory.evaluate_ind
@@ -114,28 +131,28 @@ local
   val ind_goals = ind_thm |> concl |> dest_imp |> fst |> list_dest_conj
 in
   fun get_goal s = first (can (find_term (can (match_term (Term [QUOTE s]))))) ind_goals
-  fun retcall_elim_tm () = ind_thm |> concl |> rand
+  fun ret_to_tail_tm () = ind_thm |> concl |> rand
   fun the_ind_thm () = ind_thm
 end
 
 
-Theorem retcall_elim_dec:
+Theorem ret_to_tail_Dec:
   ^(get_goal "panLang$Dec")
 Proof
-  rw [retcall_elim_def] >>
+  rw [ret_to_tail_def] >>
   fs [evaluate_def] >>
   TOP_CASE_TAC >> fs [] >>
   rpt (pairarg_tac >> fs [] >> rveq)
 QED
 
 
-Theorem retcall_elim_seq:
+Theorem ret_to_tail_Seq:
   ^(get_goal "panLang$Seq")
 Proof
-  rw [retcall_elim_def] >>
-  qmatch_goalsub_abbrev_tac ‘retcall_ret_to_tail sprog’ >>
-  ‘evaluate (retcall_ret_to_tail sprog,s) = evaluate (sprog,s)’ by (
-    ho_match_mp_tac evaluate_retcall_ret_to_tail_eq >>
+  rw [ret_to_tail_def] >>
+  qmatch_goalsub_abbrev_tac ‘seq_call_ret sprog’ >>
+  ‘evaluate (seq_call_ret sprog,s) = evaluate (sprog,s)’ by (
+    ho_match_mp_tac evaluate_seq_call_ret_eq >>
     unabbrev_all_tac >>
     imp_res_tac evaluate_seq_no_error_fst >> fs [] >>
     fs [evaluate_def] >>
@@ -149,36 +166,22 @@ Proof
   fs [evaluate_def]
 QED
 
-
-Theorem retcall_elim_if:
+Theorem ret_to_tail_If:
   ^(get_goal "panLang$If")
 Proof
-  rw [retcall_elim_def] >>
+  rw [ret_to_tail_def] >>
   fs [evaluate_def] >>
   every_case_tac >> fs [] >>
   rpt (pairarg_tac >> fs [] >> rveq)
 QED
 
-Theorem evaluate_while_no_error_imp:
-  eval s e = SOME (ValWord w) /\
-  w <> 0w /\
-  FST (evaluate (While e c,s)) <> SOME Error ==>
-  FST (evaluate (c,s)) <> SOME Error
-Proof
-  rw [] >>
-  pop_assum mp_tac >>
-  once_rewrite_tac [evaluate_def] >>
-  TOP_CASE_TAC >> fs [] >>
-  pairarg_tac >> fs [] >> rveq >>
-  every_case_tac >> fs []
-QED
-
-Theorem retcall_elim_while:
+Theorem ret_to_tail_While:
   ^(get_goal "panLang$While")
 Proof
   rw [] >>
-  fs [retcall_elim_def] >>
+  fs [ret_to_tail_def] >>
   once_rewrite_tac [evaluate_def] >>
+  TOP_CASE_TAC >> fs [] >>
   TOP_CASE_TAC >> fs [] >>
   TOP_CASE_TAC >> fs [] >>
   TOP_CASE_TAC >> fs [] >>
@@ -187,24 +190,21 @@ Proof
   disch_then (qspec_then ‘c’ mp_tac) >>
   rw [] >> fs [] >>
   rpt (pairarg_tac >> fs [] >> rveq) >>
-  TOP_CASE_TAC >> fs [] >> rveq >>
   every_case_tac >> fs [] >>
-  ‘FST (evaluate (While e c,dec_clock s1)) ≠ SOME Error’ by
+  ‘FST (evaluate (While e c,s1)) ≠ SOME Error’ by
     fs [Once evaluate_def]  >>
   fs []
 QED
 
-
-Theorem retcall_elim_call:
+Theorem ret_to_tail_Call:
   ^(get_goal "panLang$Call")
 Proof
-  rw [retcall_elim_def] >>
+  rw [ret_to_tail_def] >>
   fs [evaluate_def] >>
   every_case_tac >> fs []
 QED
 
-
-Theorem retcall_elim_others:
+Theorem ret_to_tail_Others:
   ^(get_goal "panLang$Skip") /\
   ^(get_goal "panLang$Assign") /\
   ^(get_goal "panLang$Store") /\
@@ -216,25 +216,18 @@ Theorem retcall_elim_others:
   ^(get_goal "panLang$Return") /\
   ^(get_goal "panLang$Tick")
 Proof
-  rw [retcall_elim_def]
+  rw [ret_to_tail_def]
 QED
 
-Theorem retcall_elim_correct:
-  ^(retcall_elim_tm())
+Theorem ret_to_tail_correct:
+  ^(ret_to_tail_tm())
 Proof
   match_mp_tac (the_ind_thm()) >>
-  EVERY (map strip_assume_tac [retcall_elim_dec, retcall_elim_seq,
-         retcall_elim_if, retcall_elim_while, retcall_elim_call,
-         retcall_elim_others]) >>
+  EVERY (map strip_assume_tac
+         [ret_to_tail_Dec, ret_to_tail_Seq,
+          ret_to_tail_If, ret_to_tail_While, ret_to_tail_Call,
+          ret_to_tail_Others]) >>
   asm_rewrite_tac [] >> rw [] >> rpt (pop_assum kall_tac)
-QED
-
-Theorem eval_seq_assoc_not_error:
-  FST (evaluate (p,s)) ≠ SOME Error ==>
-      FST (evaluate ((seq_assoc Skip p),s)) ≠ SOME Error
-Proof
-  rw [evaluate_seq_assoc] >>
-  rw [evaluate_def]
 QED
 
 Theorem compile_correct:
@@ -243,7 +236,7 @@ Theorem compile_correct:
 Proof
   rw [compile_prog_def] >>
   dxrule eval_seq_assoc_not_error >> strip_tac >>
-  imp_res_tac retcall_elim_correct >> fs [] >>
+  imp_res_tac ret_to_tail_correct >> fs [] >>
   rw [evaluate_seq_assoc, evaluate_def]
 QED
 
