pancake/proofs/README.md
@@ -1,5 +1,8 @@
 Proofs files for compiling Pancake.
 
+[crep_to_loopProofScript.sml](crep_to_loopProofScript.sml):
+Correctness proof for ---
+
 [loop_liveProofScript.sml](loop_liveProofScript.sml):
 Correctness proof for loop_live
 
@@ -13,4 +16,4 @@ Correctness proof for loop_to_word
 Correctness proof for pan_simp
 
 [pan_to_crepProofScript.sml](pan_to_crepProofScript.sml):
-Correctness proof for pan_simp
+Correctness proof for --
